theories/tree_borrows/defs.v
@@ -66,13 +66,14 @@ Definition init_state := (mkState ∅ ∅ {[O]} O 1).
 
 (** Tag kinds:
     - `tk_pub`: this tag is public
-    - `tk_unq_res` and `tk_unq_act`: split from the `tk_unq` in Stacked Borrows.
+    - `tk_unq tk_res` and `tk_unq tk_act`: split from the `tk_unq` in Stacked Borrows.
       We need two of them to support the two stages of 2-phase borrows.
       The intent is that whatever mutable reference is reborrowed gets a
-      `tk_unq_res` initially and on the first child write we can change it to a
-      `tk_unq_act`.
+      `tk_unq tk_res` initially and on the first child write we can change it to a
+      `tk_unq tk_act`.
     - `tk_local`: locally owned tag without any references (not even local reborrows). *)
-Inductive tag_kind := tk_pub | tk_unq_res | tk_unq_act | tk_local.
+Inductive tk_activation_kind := tk_res | tk_act.
+Inductive tag_kind := tk_pub | tk_unq (act : tk_activation_kind) | tk_local.
 
 Definition state_upd_mem (f : mem → mem) σ :=
   mkState (f σ.(shp)) σ.(strs) σ.(scs) σ.(snp) σ.(snc).
